src/riot/asn1/ASN1.Low.Value.CharacterString.fst
@@ -1,0 +1,28 @@
+module ASN1.Low.Value.CharacterString
+
+open ASN1.Low.Base
+open LowParse.Low.Bytes
+
+open ASN1.Base
+open ASN1.Low.Tag
+open ASN1.Low.Length
+open ASN1.Spec.Value.CharacterString
+include ASN1.Low.Value.StringCombinator
+include ASN1.Low.Value.IA5_STRING
+include ASN1.Low.Value.PRINTABLE_STRING
+
+open FStar.Integers
+
+module B32 = FStar.Bytes
+
+let serialize32_asn1_character_string_with_character_bound_backwards
+  (t: character_string_type)
+  (lb: asn1_value_int32_of_type t)
+  (ub: asn1_value_int32_of_type t { lb <= ub })
+: serializer32_backwards (serialize_asn1_character_string_with_character_bound t lb ub)
+= match t with
+  | IA5_STRING -> assert_norm (count_ia5_character == count_character IA5_STRING);
+                  serialize32_asn1_ia5_string_TLV_with_character_bound_backwards lb ub
+  | PRINTABLE_STRING
+               -> assert_norm (count_printable_character == count_character PRINTABLE_STRING);
+                  serialize32_asn1_printable_string_TLV_with_character_bound_backwards lb ub
