src/riot/asn1/ASN1.Spec.TLV.fst
@@ -225,3 +225,4 @@ let length_of_TLV
   (l: asn1_value_length_of_type a)
 : GTot (asn1_TLV_length_of_type a)
 = 1 + length_of_asn1_length (u l) + l
+
