src/riot/asn1/ASN1.Spec.Value.Envelop.fst
@@ -274,7 +274,11 @@ let predicate_serialize_asn1_envelop_tag_with_TLV_size
   == 1 + length_of_asn1_length len + length /\
   (* upper bound *)
   Seq.length (serialize (serialize_asn1_envelop_tag_with_TLV a s) value)
-  <= length + 6
+  <= length + 6 /\
+  Seq.length (serialize (serialize_asn1_envelop_tag_with_TLV a s) value)
+  <= asn1_TLV_length_max_of_type a /\
+  Seq.length (serialize s value)
+  <= asn1_value_length_max_of_type a
 
 let lemma_serialize_asn1_envelop_tag_with_TLV_size
   (#k: parser_kind)
