src/riot/asn1/ASN1.Spec.Value.fst
@@ -4,9 +4,10 @@ include ASN1.Spec.Value.BOOLEAN
 include ASN1.Spec.Value.NULL
 include ASN1.Spec.Value.INTEGER
 include ASN1.Spec.Value.OCTET_STRING
-include ASN1.Spec.Value.StringTypes
+include ASN1.Spec.Value.StringCombinator
 include ASN1.Spec.Value.IA5_STRING
 include ASN1.Spec.Value.PRINTABLE_STRING
+include ASN1.Spec.Value.CharacterString
 include ASN1.Spec.Value.BIT_STRING
 include ASN1.Spec.Value.OID
 include ASN1.Spec.Value.Envelop
